theories/Equivalence.v
@@ -1,7 +1,8 @@
 Require Import Coq.Classes.RelationClasses.
 Require Import Coq.Relations.Relations.
-(* Require Import Eqdep. *)
+
 Require Import Paco.paco.
+Require Import ExtLib.Structures.Monad.
 
 Require Import ITree.ITree.
 
