lib/README.md
@@ -1,6 +1,0 @@
-# Library Dependencies
-
-This lib directory should be used for 3rd-party dependencies, each of
-which can be installed independently of Vellvm:
-
-*  lib/paco  - paco-1.2.8 [available here](http://plv.mpi-sws.org/paco/)
